Generalize mem_alloc.
Now it can also be used to overwrite already allocated memory. This is useful
in the frontend, where globals can be initialized after already been allocated.
This relieves us from carrying around proofs about memory being writable.

frontend.v
@@ -560,7 +560,7 @@ Definition alloc_global (Γn : compound_env Ti) (Γ : env Ti) (m : mem Ti)
         guard (init = false) with
           ("global `" +:+ x +:+ "` already initialized");
         v ← to_init_val Γn Γ m Δg Δl τ ci;
-        inr (<[addr_top o τ:=v]{Γ}>m, <[x:=Global sto o τ true]>Δg, o, τ)
+        inr (mem_alloc Γ o false perm_full v m, <[x:=Global sto o τ true]>Δg, o, τ)
      | None => inr (m, Δg, o, τ)
      end
   | Some (Fun _ _ _ _) =>
@@ -575,12 +575,12 @@ Definition alloc_global (Γn : compound_env Ti) (Γ : env Ti) (m : mem Ti)
      let o := fresh (dom _ m) in
      match mci with
      | Some ci =>
-        let m := mem_alloc Γ o false τ m in
+        let m := mem_alloc Γ o false perm_full (val_new Γ τ) m in
         let Δg := <[x:=Global sto o τ true]>Δg in
         v ← to_init_val Γn Γ m Δg Δl τ ci;
-        inr (<[addr_top o τ:=v]{Γ}>m, Δg, o, τ)
+        inr (mem_alloc Γ o false perm_full v m, Δg, o, τ)
      | None =>
-        inr (<[addr_top o τ:=val_0 Γ τ]{Γ}>(mem_alloc Γ o false τ m),
+        inr (mem_alloc Γ o false perm_full (val_0 Γ τ) m,
              <[x:=Global sto o τ false]>Δg, o, τ)
      end
   end.
@@ -595,11 +595,11 @@ Definition alloc_static (Γn : compound_env Ti) (Γ : env Ti) (m : mem Ti)
   let Δl := Some (x,Local τ) :: Δl in
   match mci with
   | Some ci =>
-     let m := mem_alloc Γ o false τ m in
+     let m := mem_alloc Γ o false perm_full (val_new Γ τ) m in
      v ← to_init_val Γn Γ m Δg Δl τ ci;
-     inr (<[addr_top o τ:=v]{Γ}>m, o, τ)
+     inr (mem_alloc Γ o false perm_full v m, o, τ)
   | None =>
-     inr (<[addr_top o τ:=val_0 Γ τ]{Γ}>(mem_alloc Γ o false τ m), o, τ)
+     inr (mem_alloc Γ o false perm_full (val_0 Γ τ) m, o, τ)
   end.
 Definition to_storage (stos : list cstorage) : option cstorage :=
   match stos with [] => Some AutoStorage | [sto] => Some sto | _ => None end.
@@ -978,7 +978,8 @@ Hint Extern 1 (int_typed _ _) => by apply int_typed_small.
 Hint Extern 10 (cast_typed _ _ _) => constructor.
 Hint Extern 10 (base_cast_typed _ _ _) => constructor.
 Hint Extern 2 (to_funtypes _ ⊆ _) => etransitivity; [|by eassumption].
-Hint Extern 2 (_ ⇒ₘ _) => etransitivity; [|by eassumption].
+Hint Extern 2 (_ ⊆ _) => etransitivity; [|by eassumption].
+Hint Resolve memenv_subseteq_forward.
 
 Definition local_decl_valid (Γ : env Ti) (Γm : memenv Ti) (d : local_decl Ti) :=
   match d with
@@ -989,13 +990,13 @@ Definition local_decl_valid (Γ : env Ti) (Γm : memenv Ti) (d : local_decl Ti) 
 Notation local_env_valid Γ Γm := (Forall (λ xmd,
   match xmd with Some (_,d) => local_decl_valid Γ Γm d | None => True end)).
 Lemma local_decl_valid_weaken Γ1 Γ2 Γm1 Γm2 d :
-  local_decl_valid Γ1 Γm1 d → Γ1 ⊆ Γ2 → Γm1 ⇒ₘ Γm2 → local_decl_valid Γ2 Γm2 d.
+  local_decl_valid Γ1 Γm1 d → Γ1 ⊆ Γ2 → Γm1 ⊆ Γm2 → local_decl_valid Γ2 Γm2 d.
 Proof.
   destruct d; simpl; eauto using ptr_type_valid_weaken,
     type_valid_weaken, memenv_forward_typed.
 Qed.
 Lemma local_env_valid_weaken Γ1 Γ2 Γm1 Γm2 Δl :
-  local_env_valid Γ1 Γm1 Δl → Γ1 ⊆ Γ2 → Γm1 ⇒ₘ Γm2 → local_env_valid Γ2 Γm2 Δl.
+  local_env_valid Γ1 Γm1 Δl → Γ1 ⊆ Γ2 → Γm1 ⊆ Γm2 → local_env_valid Γ2 Γm2 Δl.
 Proof. induction 1 as [|[[]|]]; eauto using local_decl_valid_weaken. Qed.
 Lemma local_env_valid_params Γ Γm (ys : list string) (τs : list (type Ti)) :
   ✓{Γ}* τs → local_env_valid Γ Γm (zip_with (λ y τ, Some (y, Local τ)) ys τs).
@@ -1037,7 +1038,7 @@ Proof. induction 1 as [|[[? []]|]]; intros; simplify_option_equality; eauto. Qed
 Definition global_decl_valid (Γ : env Ti) (Γf : funtypes Ti) (Γm : memenv Ti)
     (d : global_decl Ti) :=
   match d with
-  | Global _ o τ _ => Γm ⊢ o : τ
+  | Global _ o τ _ => Γm ⊢ o : τ ∧ index_alive Γm o
   | Fun _ τs τ None =>
      ✓{Γ}* τs ∧ Forall (λ τ', int_typed (size_of Γ τ') sptrT) τs ∧ ✓{Γ} τ
   | Fun _ τs τ (Some s) => ∃ cmτ,
@@ -1052,15 +1053,15 @@ Notation global_env_valid Γ Γm Δg :=
   (map_Forall (λ _, global_decl_valid Γ (to_funtypes Δg) Γm) Δg).
 Lemma global_decl_valid_weaken Γ1 Γ2 Γf1 Γf2 Γm1 Γm2 d :
   ✓ Γ1 → global_decl_valid Γ1 Γf1 Γm1 d → Γ1 ⊆ Γ2 → Γf1 ⊆ Γf2 →
-  Γm1 ⇒ₘ Γm2 → global_decl_valid Γ2 Γf2 Γm2 d.
+  Γm1 ⊆ Γm2 → global_decl_valid Γ2 Γf2 Γm2 d.
 Proof.
   destruct d as [|??? []| |]; naive_solver eauto using
     ptr_type_valid_weaken, type_valid_weaken, memenv_forward_typed,
-    stmt_typed_weaken, types_valid_weaken, sizes_of_weaken.
+    memenv_subseteq_alive, stmt_typed_weaken, types_valid_weaken, sizes_of_weaken.
 Qed.
 Lemma global_env_valid_weaken Γ1 Γ2 Γm1 Γm2 Δg :
   ✓ Γ1 → global_env_valid Γ1 Γm1 Δg → Γ1 ⊆ Γ2 →
-  Γm1 ⇒ₘ Γm2 → global_env_valid Γ2 Γm2 Δg.
+  Γm1 ⊆ Γm2 → global_env_valid Γ2 Γm2 Δg.
 Proof. unfold map_Forall; eauto using global_decl_valid_weaken. Qed.
 Lemma global_env_empty_valid Γ Γm : global_env_valid Γ Γm ∅.
 Proof. by intros ??; simpl_map. Qed.
@@ -1154,9 +1155,8 @@ Proof.
   { eapply (lookup_var_typed _ _ _ []); eauto. }
   destruct (Δg !! x) as [d|] eqn:Hd; simplify_equality; specialize (HΔg x d Hd).
   destruct d; simplify_equality'.
-  * typed_constructor; eauto using addr_top_typed, addr_top_strict,
-      cmap_index_typed_valid, cmap_index_typed_representable,
-      lockset_empty_valid.
+  * typed_constructor; intuition eauto using addr_top_typed,lockset_empty_valid,
+      cmap_index_typed_valid, cmap_index_typed_representable, addr_top_strict.
   * typed_constructor; eauto using lockset_empty_valid.
 Qed.
 Lemma lookup_typedef_valid' Γ Γm Δg Δl x τ :
@@ -1385,17 +1385,17 @@ Proof.
   by intro; destruct (to_funtypes _ !! _); simpl_map.
 Qed.
 Lemma alloc_global_typed Γn Γ m Δg Δl x sto cτ mci m' Δg' o τ :
-  ✓ Γ → ✓{Γ} m → mem_writable_all Γ m →
+  ✓ Γ → ✓{Γ} m →
   global_env_valid Γ ('{m}) Δg → local_env_valid Γ ('{m}) Δl →
   alloc_global Γn Γ m Δg Δl x sto cτ mci = inr (m',Δg',o,τ) →
   (**i 1.) *) ✓{Γ} m' ∧
-  (**i 2.) *) mem_writable_all Γ m' ∧
-  (**i 3.) *) '{m} ⇒ₘ '{m'} ∧
-  (**i 4.) *) global_env_valid Γ ('{m'}) Δg' ∧
-  (**i 5.) *) to_funtypes Δg ⊆ to_funtypes Δg' ∧
-  (**i 6.) *) '{m'} ⊢ o : τ.
+  (**i 2.) *) '{m} ⊆ '{m'} ∧
+  (**i 3.) *) global_env_valid Γ ('{m'}) Δg' ∧
+  (**i 4.) *) to_funtypes Δg ⊆ to_funtypes Δg' ∧
+  (**i 5.) *) '{m'} ⊢ o : τ ∧
+  (**i 6.) *) index_alive ('{m'}) o.
 Proof.
-  unfold alloc_global; intros ??? HΔg ??.
+  unfold alloc_global; intros ?? HΔg ??.
   destruct (to_type Γn Γ m Δg Δl to_Type cτ) as [|τ'] eqn:?;
     simplify_equality'; case_error_guard; simplify_equality'.
   assert (✓{Γ} τ') by eauto using to_type_valid.
@@ -1404,50 +1404,48 @@ Proof.
     destruct mci as [ci|]; simplify_equality'; [|by auto 10].
     repeat case_error_guard; simplify_equality'.
     destruct (to_init_val Γn Γ m Δg Δl τ'' ci) as [v|] eqn:?; simplify_equality'.
-    assert ('{m} ⇒ₘ '{<[addr_top o τ:=v]{Γ}> m}).
-    { eapply mem_insert_forward; eauto using to_init_val_typed,
-        addr_top_typed, cmap_index_typed_representable. }
-    split_ands; eauto 8 using mem_insert_valid', to_init_val_typed,
-      addr_top_typed, cmap_index_typed_representable,
-      mem_insert_top_writable_all, global_env_insert_valid_Some,
-      global_decl_valid_weaken, memenv_forward_typed, to_funtypes_insert_Some,
-      global_env_valid_weaken. }
+    erewrite mem_alloc_alive_memenv_of by intuition eauto using to_init_val_typed.
+    split_ands; intuition eauto using global_env_insert_valid_Some,
+      to_funtypes_insert_Some, mem_alloc_alive_valid', to_init_val_typed,
+      perm_full_valid, perm_full_mapped. }
   repeat case_error_guard; simplify_equality'.
   destruct mci as [ci|]; simplify_equality'.
-  * set (m'':=mem_alloc Γ (fresh (dom indexset m)) false τ' m) in *.
+  * set (m'':=mem_alloc Γ (fresh (dom indexset m))
+      false perm_full (val_new Γ τ') m) in *.
     set (Δg'':=<[x:=Global sto (fresh (dom indexset m)) τ' true]> Δg) in *.
     destruct (to_init_val Γn Γ m'' Δg'' Δl τ' ci)
       as [v|] eqn:?; simplify_equality'.
     set (o:=fresh (dom indexset m)) in *.
-    assert (✓{Γ} m'' ∧ mem_writable_all Γ m'') as [??] by eauto using
-      mem_alloc_valid', mem_allocable_fresh, mem_alloc_writable_all.
-    assert ('{m''} ⊢ o : τ') by eauto using mem_alloc_index_typed'.
-    assert ('{m} ⇒ₘ '{m''}).
-    { eauto using mem_alloc_forward', mem_allocable_fresh. }
-    assert (global_env_valid Γ ('{m''})
-      (<[x:=Global sto (fresh (dom indexset m)) τ' true]>Δg)).
-    { eapply global_env_insert_valid; simpl; eauto using
-        global_decl_valid_weaken, global_env_valid_weaken. }
-    assert ('{m''} ⇒ₘ '{<[addr_top o τ':=v]{Γ}> m''}).
-    { eapply mem_insert_forward; eauto using to_init_val_typed, addr_top_typed,
-        index_typed_representable, local_env_valid_weaken. }
-    split_ands; eauto 8 using mem_insert_valid', to_init_val_typed,
-      addr_top_typed, index_typed_representable, mem_insert_top_writable_all,
-      memenv_forward_typed, to_funtypes_insert,
-      global_env_valid_weaken, local_env_valid_weaken.
-  * split_ands; eauto 9 using global_env_insert_valid, mem_alloc_val_valid,
-      global_env_valid_weaken, mem_alloc_val_index_typed, mem_alloc_val_forward,
-      val_0_typed, mem_allocable_fresh, to_funtypes_insert,
-      mem_alloc_val_writable_all.
+    assert (✓{Γ} m'') by eauto using mem_alloc_new_valid',
+      mem_allocable_fresh, perm_full_valid, perm_full_mapped.
+    assert ('{m''} ⊢ o : τ') by eauto using mem_alloc_new_index_typed'.
+    assert (index_alive ('{m''}) o) by eauto using mem_alloc_new_index_alive'.
+    assert ('{m} ⊆ '{m''}).
+    { unfold m''; erewrite mem_alloc_memenv_of by eauto using (val_new_typed _ ∅).
+      apply insert_subseteq, mem_allocable_memenv_of, mem_allocable_fresh. }
+    assert (global_env_valid Γ ('{m''}) (<[x:=Global sto o τ' true]> Δg)).
+    { eapply global_env_insert_valid; eauto using global_env_valid_weaken. }
+    assert (to_funtypes Δg ⊆ to_funtypes (<[x:=Global sto o τ' true]> Δg)).
+    { eauto using to_funtypes_insert. }
+    erewrite mem_alloc_alive_memenv_of
+      by intuition eauto using to_init_val_typed, local_env_valid_weaken.
+    split_ands; eauto using mem_alloc_alive_valid', to_init_val_typed,
+      perm_full_valid, perm_full_mapped, to_init_val_typed, local_env_valid_weaken.
+  * erewrite mem_alloc_memenv_of by eauto using (val_0_typed _ ∅).
+    assert ('{m} ⊆ <[fresh (dom indexset m):=(τ, false)]> ('{m})).
+    { apply insert_subseteq, mem_allocable_memenv_of, mem_allocable_fresh. }
+    split_ands; eauto 9 using global_env_insert_valid, mem_alloc_valid',
+      mem_alloc_index_alive, mem_alloc_index_typed, val_0_typed,
+      mem_allocable_fresh, to_funtypes_insert, perm_full_valid,
+      perm_full_mapped, global_env_valid_weaken.
 Qed.
 Lemma alloc_static_typed Γn Γ m Δg Δl x cτ mci m' o τ :
-  ✓ Γ → ✓{Γ} m → mem_writable_all Γ m →
+  ✓ Γ → ✓{Γ} m →
   global_env_valid Γ ('{m}) Δg → local_env_valid Γ ('{m}) Δl →
   alloc_static Γn Γ m Δg Δl x cτ mci = inr (m',o,τ) →
   (**i 1.) *) ✓{Γ} m' ∧
-  (**i 2.) *) mem_writable_all Γ m' ∧
-  (**i 3.) *) '{m} ⇒ₘ '{m'} ∧
-  (**i 4.) *) '{m'} ⊢ o : τ.
+  (**i 2.) *) '{m} ⊆ '{m'} ∧
+  (**i 3.) *) '{m'} ⊢ o : τ.
 Proof.
   unfold alloc_static; intros.
   destruct (to_type Γn Γ m Δg Δl to_Type cτ) as [|τ'] eqn:?;
@@ -1456,50 +1454,52 @@ Proof.
   repeat case_error_guard; simplify_equality'.
   destruct mci as [ci|]; simplify_equality'.
   * destruct (to_init_val Γn Γ _ Δg _ τ' ci) as [v|] eqn:?; simplify_equality'.
-    set (m'':=mem_alloc Γ (fresh (dom indexset m)) false τ m) in *.
+    set (m'':=mem_alloc Γ (fresh (dom indexset m))
+      false perm_full (val_new Γ τ) m) in *.
     set (Δl'':=Some (x, Local τ) :: Δl) in *.
     set (o:=fresh (dom indexset m)) in *.
-    assert (✓{Γ} m'' ∧ mem_writable_all Γ m'') as [??] by eauto using
-      mem_alloc_valid', mem_allocable_fresh, mem_alloc_writable_all.
-    assert ('{m''} ⊢ o : τ) by eauto using mem_alloc_index_typed'.
-    assert ('{m} ⇒ₘ '{m''}).
-    { eauto using mem_alloc_forward', mem_allocable_fresh. }
+    assert (✓{Γ} m'') by eauto using mem_alloc_new_valid',
+      mem_allocable_fresh, perm_full_valid, perm_full_mapped.
+    assert ('{m''} ⊢ o : τ) by eauto using mem_alloc_new_index_typed'.
+    assert (index_alive ('{m''}) o) by eauto using mem_alloc_new_index_alive'.
+    assert ('{m} ⊆ '{m''}).
+    { unfold m''; erewrite mem_alloc_memenv_of by eauto using (val_new_typed _ ∅).
+      apply insert_subseteq, mem_allocable_memenv_of, mem_allocable_fresh. }
     assert (local_env_valid Γ ('{m''}) Δl'').
     { constructor; eauto using local_env_valid_weaken. }
-    assert ('{m''} ⇒ₘ '{<[addr_top o τ:=v]{Γ}> m''}).
-    { eapply mem_insert_forward; eauto using to_init_val_typed, addr_top_typed,
-        index_typed_representable, global_env_valid_weaken. }
-    split_ands; eauto 8 using mem_insert_valid',
-      to_init_val_typed, addr_top_typed, mem_insert_top_writable_all,
-      memenv_forward_typed, global_env_valid_weaken.
-  * split_ands; eauto 8 using global_env_insert_valid, mem_alloc_val_valid,
-      mem_alloc_val_forward, val_0_typed, mem_allocable_fresh,
-      mem_alloc_val_writable_all, mem_alloc_val_index_typed.
+    erewrite mem_alloc_alive_memenv_of
+      by eauto using to_init_val_typed, global_env_valid_weaken.
+    split_ands; eauto using mem_alloc_alive_valid', to_init_val_typed,
+      perm_full_valid, perm_full_mapped, to_init_val_typed, global_env_valid_weaken.
+  * erewrite mem_alloc_memenv_of by eauto using (val_0_typed _ ∅).
+    assert ('{m} ⊆ <[fresh (dom indexset m):=(τ, false)]> ('{m})).
+    { apply insert_subseteq, mem_allocable_memenv_of, mem_allocable_fresh. }
+    split_ands; eauto 9 using global_env_insert_valid, mem_alloc_valid',
+      mem_alloc_index_typed, val_0_typed, mem_allocable_fresh, to_funtypes_insert,
+      perm_full_valid, perm_full_mapped, global_env_valid_weaken.
 Qed.
 Lemma to_stmt_typed Γn Γ τret m Δg Δl cs m' Δg' s cmτ :
-  ✓ Γ → ✓{Γ} m → mem_writable_all Γ m → global_env_valid Γ ('{m}) Δg →
+  ✓ Γ → ✓{Γ} m → global_env_valid Γ ('{m}) Δg →
   local_env_valid Γ ('{m}) Δl → ✓{Γ} (Some τret) →
   to_stmt Γn Γ τret m Δg Δl cs = inr (m',Δg', s,cmτ) →
   (**i 1.) *) (Γ,to_funtypes Δg','{m'},local_env_stack_types Δl) ⊢ s : cmτ ∧
   (**i 2.) *) ✓{Γ} m' ∧
-  (**i 3.) *) mem_writable_all Γ m' ∧
-  (**i 4.) *) '{m} ⇒ₘ '{m'} ∧
-  (**i 5.) *) global_env_valid Γ ('{m'}) Δg' ∧
-  (**i 6.) *) to_funtypes Δg ⊆ to_funtypes Δg'.
+  (**i 3.) *) '{m} ⊆ '{m'} ∧
+  (**i 4.) *) global_env_valid Γ ('{m'}) Δg' ∧
+  (**i 5.) *) to_funtypes Δg ⊆ to_funtypes Δg'.
 Proof.
-  intros ? Hm Hm' Hg Hl Hτret Hs.
-  revert m m' s cmτ Δl Δg Δg' Hs Hm Hm' Hg Hl.
+  intros ? Hm Hg Hl Hτret Hs. revert m m' s cmτ Δl Δg Δg' Hs Hm Hg Hl.
   induction cs; intros;
     repeat match goal with
     | H : alloc_static _ _ _ _ _ _ _ _ = inr _ |- _ =>
        first_of ltac:(apply alloc_static_typed in H) idtac ltac:(by auto);
-       destruct H as (?&?&?&?)
+       destruct H as (?&?&?)
     | H : alloc_global _ _ _ _ _ _ _ _ _ = inr _ |- _ =>
        first_of ltac:(apply alloc_global_typed in H) idtac ltac:(by auto);
        destruct H as (?&?&?&?&?&?)
     | IH : ∀ _ _ _ _ _ _ _, to_stmt _ _ _ _ _ _ ?cs = inr _ → _,
       H : to_stmt _ _ _ _ _ _ ?cs = inr _ |- _ =>
-       last_of ltac:(destruct (IH _ _ _ _ _ _ _ H) as (?&?&?&?&?&?))
+       last_of ltac:(destruct (IH _ _ _ _ _ _ _ H) as (?&?&?&?&?))
          ltac:(by eauto using local_env_valid_weaken,
            global_env_valid_weaken) ltac:(clear IH H)
     | H : to_expr _ _ _ _ _ _ = inr _ |- _ =>
@@ -1544,7 +1544,7 @@ Proof.
   * by repeat typed_constructor; eauto.
 Qed.
 Lemma to_fun_stmt_typed Γn Γ m Δg f mys τs σ cs m' Δg' s :
-  ✓ Γ → ✓{Γ} m → mem_writable_all Γ m →
+  ✓ Γ → ✓{Γ} m →
   global_env_valid Γ ('{m}) Δg → ✓{Γ} σ → ✓{Γ}* τs → length mys = length τs →
   to_fun_stmt Γn Γ m Δg f mys τs σ cs = inr (m',Δg',s) → ∃ cmτ,
   (**i 1.) *) (Γ,to_funtypes Δg','{m'},τs) ⊢ s : cmτ ∧
@@ -1552,10 +1552,9 @@ Lemma to_fun_stmt_typed Γn Γ m Δg f mys τs σ cs m' Δg' s :
   (**i 3.) *) gotos s ⊆ labels s ∧
   (**i 4.) *) throws_valid 0 s ∧
   (**i 5.) *) ✓{Γ} m' ∧
-  (**i 6.) *) mem_writable_all Γ m' ∧
-  (**i 7.) *) '{m} ⇒ₘ '{m'} ∧
-  (**i 8.) *) global_env_valid Γ ('{m'}) Δg' ∧
-  (**i 9.) *) to_funtypes Δg ⊆ to_funtypes Δg'.
+  (**i 6.) *) '{m} ⊆ '{m'} ∧
+  (**i 7.) *) global_env_valid Γ ('{m'}) Δg' ∧
+  (**i 8.) *) to_funtypes Δg ⊆ to_funtypes Δg'.
 Proof.
   unfold to_fun_stmt; intros.
   destruct (mapM id mys) as [ys|] eqn:?; simplify_equality'.
@@ -1563,7 +1562,7 @@ Proof.
   destruct (to_stmt _ _ _ _ _ _ _)
     as [|[[[m'' Δg''] s'] cmτ']] eqn:?; simplify_error_equality.
   destruct (to_stmt_typed Γn Γ σ m Δg (zip_with
-    (λ y τ, Some (y, Local τ)) ys τs) cs m'' Δg'' s' cmτ') as (Hs&?&?&?&?&?);
+    (λ y τ, Some (y, Local τ)) ys τs) cs m'' Δg'' s' cmτ') as (Hs&?&?&?&?);
     eauto using local_env_valid_params, type_valid_ptr_type_valid.
   destruct (stmt_fix_return _ s' _) as [? cmτ] eqn:?; simplify_error_equality.
   rewrite local_env_stack_types_params in Hs by done.
@@ -1575,15 +1574,14 @@ Proof.
   destruct 1; repeat constructor; auto. by apply type_valid_ptr_type_valid.
 Qed.
 Lemma alloc_fun_typed Γn Γ m Δg f sto mys cτs cτ mcs m' Δg' :
-  ✓ Γ → ✓{Γ} m → mem_writable_all Γ m → global_env_valid Γ ('{m}) Δg →
+  ✓ Γ → ✓{Γ} m → global_env_valid Γ ('{m}) Δg →
   length mys = length cτs →
   alloc_fun Γn Γ m Δg f sto mys cτs cτ mcs = inr (m',Δg') →
   (**i 1.) *) ✓{Γ} m' ∧
-  (**i 2.) *) mem_writable_all Γ m' ∧
-  (**i 3.) *) global_env_valid Γ ('{m'}) Δg' ∧
-  (**i 4.) *) to_funtypes Δg ⊆ to_funtypes Δg'.
+  (**i 2.) *) global_env_valid Γ ('{m'}) Δg' ∧
+  (**i 3.) *) to_funtypes Δg ⊆ to_funtypes Δg'.
 Proof.
-  unfold alloc_fun. intros ??? HΔg ? Halloc.
+  unfold alloc_fun. intros ?? HΔg ? Halloc.
   destruct (fmap _ <$> mapM _ _) as [|τs] eqn:?; simplify_equality'.
   assert (✓{Γ}* τs ∧ length mys = length τs) as [].
   { clear Halloc. destruct (mapM _ _) as [|σs] eqn:?; simplify_equality'. split.
@@ -1600,7 +1598,7 @@ Proof.
     destruct (to_fun_stmt _ _ _ _ _ _ _ _ _)
       as [|[[m'' Δg''] s]] eqn:?; simplify_equality'.
     destruct (to_fun_stmt_typed Γn Γ m Δg f mys τs σ cs m' Δg'' s)
-      as (mcσ&?&?&?&?&?&?&?&?&?); auto.
+      as (mcσ&?&?&?&?&?&?&?&?); auto.
     destruct (lookup_to_funtypes_1 Δg'' f τs σ)
       as (sto''&mcτ&?); eauto using lookup_weaken.
     set (sto''' := if decide (sto = ExternStorage) then sto' else sto).
@@ -1617,7 +1615,7 @@ Proof.
     assert (to_funtypes Δg ⊆ to_funtypes Δg').
       by eauto 10 using to_funtypes_insert.
     destruct (to_fun_stmt_typed Γn Γ m Δg' f mys τs σ cs m' Δg'' s)
-      as (mcσ&?&?&?&?&?&?&?&?&?); eauto 10 using global_env_insert_valid.
+      as (mcσ&?&?&?&?&?&?&?&?); eauto 10 using global_env_insert_valid.
     destruct (lookup_to_funtypes_1 Δg'' f τs σ) as (?&?&?).
     { eapply lookup_weaken; eauto.
       by unfold Δg'; eapply lookup_to_funtypes_2; simpl_map. }
@@ -1646,35 +1644,33 @@ Proof.
       eauto using global_env_insert_valid, to_funtypes_insert.
 Qed.
 Lemma to_envs_go_typed Θ Γn Γ m Δg Γn' Γ' m' Δg' :
-  ✓ Γ → ✓{Γ} m → mem_writable_all Γ m → global_env_valid Γ ('{m}) Δg →
+  ✓ Γ → ✓{Γ} m → global_env_valid Γ ('{m}) Δg →
   to_envs_go Γn Γ m Δg Θ = inr (Γn',Γ',m',Δg') →
   (**i 1.) *) ✓ Γ' ∧
   (**i 2.) *) ✓{Γ'} m' ∧
-  (**i 3.) *) mem_writable_all Γ' m' ∧
-  (**i 4.) *) global_env_valid Γ' ('{m'}) Δg' ∧
-  (**i 5.) *) to_funtypes Δg ⊆ to_funtypes Δg'.
+  (**i 3.) *) global_env_valid Γ' ('{m'}) Δg' ∧
+  (**i 4.) *) to_funtypes Δg ⊆ to_funtypes Δg'.
 Proof.
   revert Γn Γ m Δg.
   induction Θ as [|[x [c cτys|cτi yces|cτ|stos cτ mce|stos cτys cσ mcs]] Θ IH];
-    intros Γn Γ m Δg ?????; simplify_equality'.
+    intros Γn Γ m Δg ????; simplify_equality'.
   * done.
   * destruct (mapM _ _) as [|τs] eqn:?; simplify_error_equality.
     assert (✓ (<[x:tag:=τs]> Γ)) by (constructor; eauto using to_types_valid).
     apply (IH (<[(x:tag):=CompoundType c (fst <$> cτys)]>Γn)
       (<[(x:tag):=τs]>Γ) m Δg); simpl in *; auto.
     + eauto using cmap_valid_weaken', insert_subseteq.
-    + eauto using mem_writable_all_weaken, insert_subseteq.
     + eauto using global_env_valid_weaken, insert_subseteq.
   * repeat case_error_guard; simplify_equality'.
     destruct (to_enum Γn Γ m (to_inttype cτi) Δg yces 0)
       as [|Δg''] eqn:?; simplify_equality'.
     destruct (to_enum_typed Γn Γ m (to_inttype cτi) Δg yces 0 Δg''); eauto.
     destruct (IH (<[x:tag:=EnumType (to_inttype cτi)]> Γn) Γ m Δg'')
-      as (?&?&?&?&?); eauto 10.
+      as (?&?&?&?); eauto 10.
   * repeat case_error_guard; simplify_equality'.
     destruct (to_type _ _ _ _ _ _ _) as [τ|] eqn:?; simplify_equality'.
     destruct (IH Γn Γ m (<[x:=GlobalTypeDef t]> Δg))
-      as (?&?&?&?&?); eauto 7 using global_env_insert_valid,
+      as (?&?&?&?); eauto 7 using global_env_insert_valid,
       to_ptr_type_valid, to_funtypes_insert.
   * repeat case_error_guard; simplify_equality'.
     destruct (to_storage _) as [sto|]; simplify_equality'.
@@ -1682,15 +1678,15 @@ Proof.
       as [|[[[m'' Δg''] o] τ]] eqn:?; simplify_equality'.
     destruct (alloc_global_typed Γn Γ m Δg [] x sto cτ mce m'' Δg'' o τ)
       as (?&?&?&?&?&?); eauto using to_type_valid.
-    destruct (IH Γn Γ m'' Δg'') as (?&?&?&?&?);
+    destruct (IH Γn Γ m'' Δg'') as (?&?&?&?);
       eauto 10 using global_env_valid_weaken.
   * repeat case_error_guard; simplify_equality'.
     destruct (to_storage _) as [sto|]; simplify_equality'.
     destruct (alloc_fun _ _ _ _ _ _ _ _ _ _)
       as [|[m'' Δg'']] eqn:?; simplify_error_equality.
     destruct (alloc_fun_typed Γn Γ m Δg x sto (fst <$> cτys) (snd <$> cτys)
-      cσ mcs m'' Δg'') as (?&?&?&?); rewrite ?fmap_length; eauto.
-    destruct (IH Γn Γ m'' Δg'') as (?&?&?&?&?);
+      cσ mcs m'' Δg'') as (?&?&?); rewrite ?fmap_length; eauto.
+    destruct (IH Γn Γ m'' Δg'') as (?&?&?&?);
       eauto 10 using global_env_valid_weaken.
 Qed.
 Lemma to_envs_typed Θ Γn Γ m Δg :
@@ -1698,13 +1694,12 @@ Lemma to_envs_typed Θ Γn Γ m Δg :
   (**i 1.) *) ✓ Γ ∧
   (**i 2.) *) ✓{Γ} (to_funtypes Δg) ∧
   (**i 3.) *) (Γ,'{m}) ⊢ to_funenv Δg : to_funtypes Δg ∧
-  (**i 4.) *) ✓{Γ} m ∧
-  (**i 5.) *) mem_writable_all Γ m.
+  (**i 4.) *) ✓{Γ} m.
 Proof.
   unfold to_envs. intros. destruct (to_envs_go _ _ _ _ _)
     as [|[[[??] ?] ?]] eqn:?; simplify_error_equality.
   destruct (to_envs_go_typed Θ ∅ ∅ ∅ ∅ Γn Γ m Δg)
-    as (?&?&?&?&?); eauto 6 using env_empty_valid, mem_writable_all_empty,
+    as (?&?&?&?); eauto 6 using env_empty_valid,
     cmap_empty_valid, to_funenv_typed, global_env_empty_valid.
 Qed.
 End properties.
